Fiddled with linking

memmgr/main.c
@@ -49,7 +49,7 @@ int main(void) {
   printf("done\n");
 */
 
-  printf("short test done\n");
+/*  printf("short test done\n"); */
 
   return 0;
 }
