memmgr/verif_external.v
@@ -4,15 +4,23 @@ Require Import malloc_lemmas.
 Require Import mmap0.
 Require Import spec_malloc.
 Require Import linking.
+Require Import spec_external.
 
+Definition Gprog : funspecs := [placeholder_spec].
+
+Lemma body_placeholder: semax_body Vprog Gprog f_placeholder spec_external.placeholder_spec.
+Proof.
+start_function.
+contradiction.
+Qed.
 
 Parameter body_mmap0:
  forall {Espec: OracleKind} {cs: compspecs},
   VST.floyd.library.body_lemma_of_funspec
     (EF_external "mmap0"
 (* TODO Tint for size_t and off_t *)
-       {| sig_args := AST.Tptr :: AST.Tint::AST.Tint::AST.Tint::AST.Tint::AST.Tint::nil;
-          sig_res := None; sig_cc := cc_default |})
+       {| sig_args := AST.Tptr :: AST.Tint::AST.Tint::AST.Tint::AST.Tint::AST.Tlong::nil;
+          sig_res := Some AST.Tint; sig_cc := cc_default |})
     (snd mmap0_spec).
 
 Parameter body_munmap:
@@ -74,5 +82,6 @@ Existing Instance NullExtension.Espec.
 
 Definition module : list semax_body_proof := 
  [mk_external mmap0._mmap0 (tptr tvoid) tcret_mmap0 body_mmap0;
-  mk_external mmap0._munmap tint tcret_munmap body_munmap].
+  mk_external mmap0._munmap tint tcret_munmap body_munmap;
+  mk_body body_placeholder].
 
