memmgr/verif_fill_bin.v
@@ -6,7 +6,7 @@ Require Import malloc.
 Require Import spec_malloc.
 Require Import linking. (* just for mk_body *)
 
-Definition Gprog : funspecs := user_specs ++ private_specs.
+Definition Gprog : funspecs := external_specs ++ user_specs ++ private_specs.
 
 (* Invariant for loop in fill_bin.
 p, s, N are fixed
@@ -344,7 +344,7 @@ It would be nice to factor commonalities. *)
        apply (malloc_compat_WORD_q N j (Vptr pblk poff)); auto; try rep_omega.
        subst s; apply bin2size_align; auto.
     ** destruct H5 as [H5a [H5j H5align]]; normalize.
-    ** entailer!.  
+    ** entailer!.
   }
   Intros. (* flattens the SEP clause *) 
   freeze [0;5] Fwaste. (* discard what's not needed for post *)
