memmgr/verif_malloc_large.v
@@ -4,7 +4,7 @@ Require Import malloc.
 Require Import spec_malloc.
 Require Import linking.
 
-Definition Gprog : funspecs := user_specs ++ private_specs.
+Definition Gprog : funspecs := external_specs ++ user_specs ++ private_specs.
 
 Lemma body_malloc_large: semax_body Vprog Gprog f_malloc_large malloc_large_spec.
 Proof.
