memmgr/mmap0.v
@@ -3,12 +3,12 @@ From compcert Require Import Coqlib Integers Floats AST Ctypes Cop Clight Clight
 Local Open Scope Z_scope.
 
 Module Info.
-  Definition version := "3.4"%string.
+  Definition version := "3.5"%string.
   Definition build_number := ""%string.
   Definition build_tag := ""%string.
   Definition arch := "x86"%string.
   Definition model := "32sse2"%string.
-  Definition abi := "macosx"%string.
+  Definition abi := "standard"%string.
   Definition bitsize := 32.
   Definition big_endian := false.
   Definition source_file := "mmap0.c"%string.
@@ -66,47 +66,10 @@ Definition ___compcert_va_composite : ident := 17%positive.
 Definition ___compcert_va_float64 : ident := 16%positive.
 Definition ___compcert_va_int32 : ident := 14%positive.
 Definition ___compcert_va_int64 : ident := 15%positive.
-Definition _addr : ident := 54%positive.
-Definition _fildes : ident := 58%positive.
-Definition _flags : ident := 57%positive.
-Definition _len : ident := 55%positive.
-Definition _main : ident := 63%positive.
-Definition _mmap : ident := 52%positive.
-Definition _mmap0 : ident := 61%positive.
-Definition _munmap : ident := 53%positive.
-Definition _off : ident := 59%positive.
-Definition _p : ident := 60%positive.
-Definition _placeholder : ident := 62%positive.
-Definition _prot : ident := 56%positive.
-Definition _t'1 : ident := 64%positive.
-
-Definition f_mmap0 := {|
-  fn_return := (tptr tvoid);
-  fn_callconv := cc_default;
-  fn_params := ((_addr, (tptr tvoid)) :: (_len, tuint) :: (_prot, tint) ::
-                (_flags, tint) :: (_fildes, tint) :: (_off, tlong) :: nil);
-  fn_vars := nil;
-  fn_temps := ((_p, (tptr tvoid)) :: (_t'1, (tptr tvoid)) :: nil);
-  fn_body :=
-(Ssequence
-  (Ssequence
-    (Scall (Some _t'1)
-      (Evar _mmap (Tfunction
-                    (Tcons (tptr tvoid)
-                      (Tcons tuint
-                        (Tcons tint
-                          (Tcons tint (Tcons tint (Tcons tlong Tnil))))))
-                    (tptr tvoid) cc_default))
-      ((Etempvar _addr (tptr tvoid)) :: (Etempvar _len tuint) ::
-       (Etempvar _prot tint) :: (Etempvar _flags tint) ::
-       (Etempvar _fildes tint) :: (Etempvar _off tlong) :: nil))
-    (Sset _p (Etempvar _t'1 (tptr tvoid))))
-  (Sifthenelse (Ebinop Oeq (Etempvar _p (tptr tvoid))
-                 (Ecast (Eunop Oneg (Econst_int (Int.repr 1) tint) tint)
-                   (tptr tvoid)) tint)
-    (Sreturn (Some (Ecast (Econst_int (Int.repr 0) tint) (tptr tvoid))))
-    (Sreturn (Some (Etempvar _p (tptr tvoid))))))
-|}.
+Definition _main : ident := 55%positive.
+Definition _mmap0 : ident := 53%positive.
+Definition _munmap : ident := 52%positive.
+Definition _placeholder : ident := 54%positive.
 
 Definition f_placeholder := {|
   fn_return := tint;
@@ -363,8 +326,13 @@ Definition global_definitions : list (ident * globdef fundef type) :=
                      {|cc_vararg:=true; cc_unproto:=false; cc_structret:=false|}))
      (Tcons tint Tnil) tvoid
      {|cc_vararg:=true; cc_unproto:=false; cc_structret:=false|})) ::
- (_mmap,
-   Gfun(External (EF_external "mmap"
+ (_munmap,
+   Gfun(External (EF_external "munmap"
+                   (mksignature (AST.Tint :: AST.Tint :: nil) (Some AST.Tint)
+                     cc_default)) (Tcons (tptr tvoid) (Tcons tuint Tnil))
+     tint cc_default)) ::
+ (_mmap0,
+   Gfun(External (EF_external "mmap0"
                    (mksignature
                      (AST.Tint :: AST.Tint :: AST.Tint :: AST.Tint ::
                       AST.Tint :: AST.Tlong :: nil) (Some AST.Tint)
@@ -373,33 +341,27 @@ Definition global_definitions : list (ident * globdef fundef type) :=
        (Tcons tuint
          (Tcons tint (Tcons tint (Tcons tint (Tcons tlong Tnil))))))
      (tptr tvoid) cc_default)) ::
- (_munmap,
-   Gfun(External (EF_external "munmap"
-                   (mksignature (AST.Tint :: AST.Tint :: nil) (Some AST.Tint)
-                     cc_default)) (Tcons (tptr tvoid) (Tcons tuint Tnil))
-     tint cc_default)) :: (_mmap0, Gfun(Internal f_mmap0)) ::
  (_placeholder, Gfun(Internal f_placeholder)) :: nil).
 
 Definition public_idents : list ident :=
-(_placeholder :: _mmap0 :: _munmap :: _mmap :: ___builtin_debug ::
- ___builtin_nop :: ___builtin_write32_reversed ::
- ___builtin_write16_reversed :: ___builtin_read32_reversed ::
- ___builtin_read16_reversed :: ___builtin_fnmsub :: ___builtin_fnmadd ::
- ___builtin_fmsub :: ___builtin_fmadd :: ___builtin_fmin ::
- ___builtin_fmax :: ___builtin_ctzll :: ___builtin_ctzl :: ___builtin_ctz ::
- ___builtin_clzll :: ___builtin_clzl :: ___builtin_clz ::
- ___builtin_bswap64 :: ___compcert_i64_umulh :: ___compcert_i64_smulh ::
- ___compcert_i64_sar :: ___compcert_i64_shr :: ___compcert_i64_shl ::
- ___compcert_i64_umod :: ___compcert_i64_smod :: ___compcert_i64_udiv ::
- ___compcert_i64_sdiv :: ___compcert_i64_utof :: ___compcert_i64_stof ::
- ___compcert_i64_utod :: ___compcert_i64_stod :: ___compcert_i64_dtou ::
- ___compcert_i64_dtos :: ___compcert_va_composite ::
- ___compcert_va_float64 :: ___compcert_va_int64 :: ___compcert_va_int32 ::
- ___builtin_va_end :: ___builtin_va_copy :: ___builtin_va_arg ::
- ___builtin_va_start :: ___builtin_membar :: ___builtin_annot_intval ::
- ___builtin_annot :: ___builtin_memcpy_aligned :: ___builtin_fsqrt ::
- ___builtin_fabs :: ___builtin_bswap16 :: ___builtin_bswap32 ::
- ___builtin_bswap :: nil).
+(_placeholder :: _mmap0 :: _munmap :: ___builtin_debug :: ___builtin_nop ::
+ ___builtin_write32_reversed :: ___builtin_write16_reversed ::
+ ___builtin_read32_reversed :: ___builtin_read16_reversed ::
+ ___builtin_fnmsub :: ___builtin_fnmadd :: ___builtin_fmsub ::
+ ___builtin_fmadd :: ___builtin_fmin :: ___builtin_fmax ::
+ ___builtin_ctzll :: ___builtin_ctzl :: ___builtin_ctz :: ___builtin_clzll ::
+ ___builtin_clzl :: ___builtin_clz :: ___builtin_bswap64 ::
+ ___compcert_i64_umulh :: ___compcert_i64_smulh :: ___compcert_i64_sar ::
+ ___compcert_i64_shr :: ___compcert_i64_shl :: ___compcert_i64_umod ::
+ ___compcert_i64_smod :: ___compcert_i64_udiv :: ___compcert_i64_sdiv ::
+ ___compcert_i64_utof :: ___compcert_i64_stof :: ___compcert_i64_utod ::
+ ___compcert_i64_stod :: ___compcert_i64_dtou :: ___compcert_i64_dtos ::
+ ___compcert_va_composite :: ___compcert_va_float64 ::
+ ___compcert_va_int64 :: ___compcert_va_int32 :: ___builtin_va_end ::
+ ___builtin_va_copy :: ___builtin_va_arg :: ___builtin_va_start ::
+ ___builtin_membar :: ___builtin_annot_intval :: ___builtin_annot ::
+ ___builtin_memcpy_aligned :: ___builtin_fsqrt :: ___builtin_fabs ::
+ ___builtin_bswap16 :: ___builtin_bswap32 :: ___builtin_bswap :: nil).
 
 Definition prog : Clight.program := 
   mkprogram composites global_definitions public_idents _main Logic.I.
